theories/stacked_borrows/examples/opt2.v
@@ -1,4 +1,6 @@
+From simuliris.simulation Require Import lifting.
 From simuliris.stacked_borrows Require Import proofmode lang.
+
 Set Default Proof Using "Type".
 
 (** Moving read of shared ref up across code that *may* use that ref. *)
@@ -14,22 +16,14 @@ Definition ex2_unopt : ectx :=
     (* (x, Tagged pid_x) ↦{tk_local} i *)
 
     (* retag_place reborrows the pointer value stored in "x" (which is "i"),
-      then updates "x" with the new pointer value. A [Default] retag is
-      sufficient for this, we don't need the protector. *)
-    retag_place "x" (RefPtr Immutable) int Default "c";;
-    (* (x, Tagged pid_x) ↦{tk_local} ScPtr l t 
-       (l, Tagged npid) ↦{tk_shr} v
+      then updates "x" with the new pointer value.
+      Using a protector here.
     *)
+    retag_place "x" (RefPtr Immutable) int FnEntry "c";;
 
     (* The unknown code is represented by a call to an unknown function "f",
       which does take the pointer value from "x" as an argument. *)
     Call #[ScFnPtr "f"] (Copy "x") ;;
-    (* need to insert x into the bijection for the call.
-        point: for this to work, we need to retain some knowledge about the value even beyond the bijection.
-        i.e.: retain a fractional points-to!
-
-        (l, Tagged npid) ↦{q, tk_shr} v
-    *)
 
     (* Read the value "v" from the cell pointed to by the pointer in "x" *)
     let: "v" := Copy *{int} "x" in
@@ -46,20 +40,109 @@ Definition ex2_opt : ectx :=
   λ: "i",
     let: "c" := InitCall in
     let: "x" := new_place (& int) "i" in
-    retag_place "x" (RefPtr Immutable) int Default "c";;
+    retag_place "x" (RefPtr Immutable) int FnEntry "c";;
     let: "v" := Copy *{int} "x" in
-    (* NOTE: here we have the same problem as in opt1.v: we need to know that the stack has not changed. 
-        moreover: might need to keep track of the type/type size somewhere?*)
     Call #[ScFnPtr "f"] (Copy "x") ;;
     Free "x" ;;
     EndCall "c";;
     "v"
   .
 
+Lemma sim_opt2 `{sborG Σ} π :
+  ⊢ sim_ectx rrel π ex2_opt ex2_unopt rrel.
+Proof.
+  iIntros (r_t r_s) "Hrel".
+  sim_pures.
+  sim_apply InitCall InitCall (sim_initcall) "". iIntros (c) "Hcall". iApply sim_expr_base. sim_pures.
 
-(* NOTE regarding allocation size: just weaken that to say that it either has a size or has been deallocated.
-  Then we should be able to make that token persistent. 
-  (we can rule out the "deallocated" case with a pointsto, if needed) 
-*)
+  sim_apply (Alloc _) (Alloc _) sim_alloc_local "". iIntros (t l_t l_s) "Htag Ht Hs".
+  iApply sim_expr_base. sim_pures.
+
+  source_bind (Write _ _).
+  destruct r_s as [v_s | ]; first last.
+  { iApply source_red_irred_unless; first done. by iIntros. }
+  (* gain knowledge about the length *)
+  iApply source_red_irred_unless; first done. iIntros (Hsize).
+  iApply (source_write_local with "Htag Hs"); [by rewrite repeat_length | done | ].
+  iIntros "Hs Htag". source_finish.
+  iPoseProof (rrel_value_source with "Hrel") as (v_t) "(-> & #Hv)".
+  iPoseProof (value_rel_length with "Hv") as "%Hlen".
+  target_apply (Write _ _) (target_write_local with "Htag Ht") "Ht Htag"; [ by rewrite repeat_length | lia| ].
+  sim_pures.
+
+  target_apply (Copy _) (target_copy_local with "Htag Ht") "Ht Htag"; first lia.
+  source_apply (Copy _) (source_copy_local with "Htag Hs") "Hs Htag"; first lia.
+
+  (* do the retag *)
+  sim_bind (Retag _ _ _ _ _) (Retag _ _ _ _ _).
+  iApply sim_irred_unless; first done.
+  iIntros ((_ & ot & i & -> & _)).
+  iPoseProof (value_rel_singleton_source with "Hv") as (sc_t) "[-> Hscrel]".
+  iPoseProof (sc_rel_ptr_source with "Hscrel") as "[-> Htagged]".
+  iApply (sim_retag_fnentry with "Hscrel Hcall"); [cbn; lia|  ].
+  iIntros (t_i v_t v_s Hlen_t Hlen_s) "Hvrel Hcall Htag_i Hi_t Hi_s #Hsc_i".
+  iApply sim_expr_base.
+  target_apply (Write _ _) (target_write_local with "Htag Ht") "Ht Htag"; [done | done | ].
+  source_apply (Write _ _) (source_write_local with "Htag Hs") "Hs Htag"; [done | done | ].
+  sim_pures.
+
+  (* read in the target *)
+  target_apply (Copy (Place _ _ _)) (target_copy_local with "Htag Ht") "Ht Htag"; first done.
+  target_pures. target_apply (Copy _) (target_copy_protected with "Hcall Htag_i Hi_t") "Hi_t Hcall Htag_i"; [done | | ].
+  { simpl. intros i0 Hi0. assert (i0 = O) as -> by lia. eexists. split; first apply lookup_insert. set_solver. }
+
+  sim_pures. target_apply (Copy _) (target_copy_local with "Htag Ht") "Ht Htag"; first done.
+  source_apply (Copy _) (source_copy_local with "Htag Hs") "Hs Htag"; first done. sim_pures.
+  sim_apply (Call _ _) (Call _ _) (sim_call _ _ (ValR [ScPtr i _]) (ValR [ScPtr i _])) "".
+  { iApply big_sepL2_singleton. iApply "Hsc_i". }
+  iIntros (r_t r_s) "_". sim_pures.
+
+  (* read in the source *)
+  source_apply (Copy (Place _ _ _)) (source_copy_local with "Htag Hs") "Hs Htag"; first done.
+  source_pures. source_apply (Copy _) (source_copy_any with "Htag_i Hi_s") "Hi_s Htag_i"; first done.
+  sim_pures.
+
+  sim_bind (Free _) (Free _).
+  (* TODO: need local free lemma that also removes the ghost state for that *)
+Abort.
 
 
+
+
+(* TODO: use LLVM read semantics for the following optimization *)
+(* Assuming x : & i32 *)
+Definition ex2_unopt' : ectx :=
+  λ: "i",
+    (* "x" is the local variable that stores the pointer value "i" *)
+    let: "x" := new_place (& int) "i" in
+    (* (x, Tagged pid_x) ↦{tk_local} i *)
+
+    (* retag_place reborrows the pointer value stored in "x" (which is "i"),
+      then updates "x" with the new pointer value. A [Default] retag is
+      sufficient for this, we don't need the protector. *)
+    retag_place "x" (RefPtr Immutable) int Default #[ScCallId 0];;
+
+    (* The unknown code is represented by a call to an unknown function "f",
+      which does take the pointer value from "x" as an argument. *)
+    Call #[ScFnPtr "f"] (Copy "x") ;;
+
+    (* Read the value "v" from the cell pointed to by the pointer in "x" *)
+    let: "v" := Copy *{int} "x" in
+
+    (* Free the local variable *)
+    Free "x" ;;
+
+    (* Finally, return the read value *)
+    EndCall "c";;
+    "v"
+  .
+
+Definition ex2_opt' : ectx :=
+  λ: "i",
+    let: "x" := new_place (& int) "i" in
+    retag_place "x" (RefPtr Immutable) int Default #[ScCallId 0];;
+    let: "v" := Copy *{int} "x" in
+    Call #[ScFnPtr "f"] (Copy "x") ;;
+    Free "x" ;;
+    "v"
+  .
