theories/stacked_borrows/examples/opt1_down.v
@@ -1,4 +1,5 @@
-From simuliris.stacked_borrows Require Import proofmode lang.
+From simuliris.simulation Require Import lifting.
+From simuliris.stacked_borrows Require Import proofmode defs lang heap.
 Set Default Proof Using "Type".
 
 (** Moving a read of a mutable reference down across code that *may* use that ref. *)
@@ -42,5 +43,60 @@ Definition ex1_down_opt : ectx :=
     EndCall "c";;
     "v"
   .
+
+Lemma sim_opt1_down `{sborG Σ} π :
+  ⊢ sim_ectx rrel π ex1_down_opt ex1_down_unopt rrel.
+Proof.
+  iIntros (r_t r_s) "Hrel".
+  sim_pures.
+  sim_apply InitCall InitCall sim_initcall "". iIntros (c) "Hcall". iApply sim_expr_base. sim_pures.
+  sim_apply (Alloc _) (Alloc _) sim_alloc_local "". iIntros (t l_t l_s) "Htag Ht Hs".
+  iApply sim_expr_base. sim_pures. simpl.
+
+  source_bind (Write _ _).
+  destruct r_s as [v_s | ]; first last.
+  { iApply source_red_irred_unless; first done. by iIntros. }
+  (* gain knowledge about the length *)
+  iApply source_red_irred_unless; first done. iIntros (Hsize). simpl.
+  iApply (source_write_local with "Htag Hs"); [ done | done | ].
+  iIntros "Hs Htag". source_finish.
+  iPoseProof (rrel_value_source with "Hrel") as (v_t) "(-> & #Hv)".
+  iPoseProof (value_rel_length with "Hv") as "%Hlen".
+  target_apply (Write _ _) (target_write_local with "Htag Ht") "Ht Htag"; [ done | lia| ].
+  sim_pures.
+
+  target_apply (Copy _) (target_copy_local with "Htag Ht") "Ht Htag"; first lia.
+  source_apply (Copy _) (source_copy_local with "Htag Hs") "Hs Htag"; first lia.
+
+  (* do the retag *)
+  sim_bind (Retag _ _ _ _ _) (Retag _ _ _ _ _).
+  iApply sim_irred_unless; first done.
+  iIntros ((_ & ot & i & -> & _)).
+  iPoseProof (value_rel_singleton_source with "Hv") as (sc_t) "[-> Hscrel]".
+  iPoseProof (sc_rel_ptr_source with "Hscrel") as "[-> Htagged]". 
+  iApply (sim_retag_fnentry with "Hscrel Hcall"); [cbn; lia| ].
+  iIntros (t_i v_t v_s Hlen_t Hlen_s) "Hvrel Hcall Htag_i Hi_t Hi_s _".
+  iApply sim_expr_base.
+  target_apply (Write _ _) (target_write_local with "Htag Ht") "Ht Htag"; [done | done | ].
+  source_apply (Write _ _) (source_write_local with "Htag Hs") "Hs Htag"; [done | done | ].
+  sim_pures.
+
+  (* do the source load *)
+  source_apply (Copy (Place _ _ _)) (source_copy_local with "Htag Hs") "Hs Htag"; first done.
+  source_pures. source_apply (Copy _) (source_copy_any with "Htag_i Hi_s") "Hi_s Htag_i"; first done. 
+  sim_pures.
+
+  sim_apply (Call _ _) (Call _ _) (sim_call _ _ (ValR []) (ValR [])) ""; first by iApply value_rel_empty.
+  iIntros (r_t r_s) "_". sim_pures.
+
+  (* do the target load *)
+  target_apply (Copy (Place _ _ _)) (target_copy_local with "Htag Ht") "Ht Htag"; first done.
+  target_pures. target_apply (Copy _) (target_copy_protected with "Hcall Htag_i Hi_t") "Hi_t Hcall Htag_i"; first done.
+  { simpl. intros i0 Hi0. assert (i0 = O) as -> by lia. eexists. split; first apply lookup_insert.  set_solver. } 
+  sim_pures. 
+
+  sim_bind (Free _) (Free _).
+  (* TODO: need local free lemma that also removes the ghost state for that *)
+Abort.
 
 
